src/QUIC.Parse.fsti
@@ -1,0 +1,8 @@
+module QUIC.Parse
+
+module B = LowStar.Buffer
+module U8 = FStar.UInt8
+module U32 = FStar.UInt32
+module HST = FStar.HyperStack.ST
+
+val test : B.buffer U8.t -> HST.Stack U32.t (requires (fun _ -> False)) (ensures (fun _ _ _ -> True))
